newio/PDM.IO.Respects.fst
@@ -1,0 +1,225 @@
+module PDM.IO.Respects
+
+open FStar.Classical.Sugar
+open FStar.List.Tot.Base
+open FStar.Tactics
+
+open Free
+open Free.IO
+open Hist
+open DM.IO
+open DM.IO.Refine
+
+let pdm (a:Type) (wp:hist a) = 
+  pre : pure_pre { forall p h. wp p h ==> pre } & (squash pre -> dm a wp)
+
+let get_pre (t : pdm 'a 'wp) : Pure pure_pre (requires True) (ensures fun r -> forall post hist. 'wp post hist ==> r) =
+  let (| pre , f |) = t in pre
+
+let get_fun (t : pdm 'a 'wp) : Pure (dm 'a 'wp) (requires get_pre t) (ensures fun _ -> True) =
+  let (| pre, f |) = t in f ()
+
+
+(*** Defining the predicate needed, respects **)
+(** the post-condition is written over an output value and local trace, therefore,
+  `return_of` is not enough and we need predicates and lemmas that show that for 
+  each x that is a returned value by m, also exists a local trace **)
+  
+let rec trace_of (lt:trace) (m:io 'a) (x:'a) =
+  match lt, m with
+  | [], Return x' -> x == x'
+  | e::es, Call cmd arg k -> 
+     (let (| cmd', arg', res' |) = destruct_event e in 
+          (cmd' == cmd /\ arg == arg' /\ (trace_of es (k res') x)))
+  | _, _ -> False
+
+let exists_trace_of (x:'a) (m:io 'a) =
+  exists lt. trace_of lt m x
+
+let rec lemma_return_of_implies_exists_trace_of (m:io 'a) (x:'a) : 
+  Lemma
+    (requires (x `return_of` m))
+    (ensures (exists_trace_of x m)) =
+  match m with
+  | Return _ -> assert (trace_of [] m x)
+  | Call cmd arg k -> begin
+    eliminate exists r. (x `return_of` (k r)) returns (exists_trace_of x m) with _. begin
+      lemma_return_of_implies_exists_trace_of (k r) x;
+      assert (exists klt. trace_of klt (k r) x) by (assumption ());
+      eliminate exists klt. trace_of klt (k r) x returns (exists_trace_of x m) with _. begin
+        let e = convert_call_to_event cmd arg r in
+        introduce exists lt. (trace_of lt m x) with (e::klt) and begin
+          assert (trace_of (e::klt) m x)
+        end
+      end
+    end
+  end
+
+let rec lemma_theta_result_implies_post m p h : 
+  Lemma 
+    (requires theta m p h) 
+    (ensures (forall x lt. trace_of lt m x ==> p lt x)) =
+  introduce forall x lt. trace_of lt m x ==> p lt x with begin
+    introduce trace_of lt m x ==> p lt x with _. begin
+      match m with
+      | Return _ -> ()
+      | Call cmd arg k -> begin
+        let e::klt = lt in
+        let (| cmd', arg', res' |) = destruct_event e in
+        lemma_theta_result_implies_post (k res') (hist_post_shift p [convert_call_to_event cmd arg res']) (convert_call_to_event cmd arg res' :: h);
+        assert (trace_of klt (k res') x);
+        assert (hist_post_shift p [convert_call_to_event cmd arg res'] klt x)
+      end
+    end
+  end
+
+(** here is Theo's idea with respects **)
+let respects (x:'a) (d:dm 'a 'wp) : Type0 =
+  forall (h:trace) (p:hist_post #event 'a). 'wp p h ==> (exists (lt:trace). p lt x)
+
+(** and we show that return_of implies respects **)
+let lemma_return_of_implies_respects (d:dm 'a 'wp) :
+  Lemma (forall x. x `return_of` d ==> x `respects` d) = 
+  assert ('wp `hist_ord` theta d);
+  introduce forall x. x `return_of` d ==> x `respects` d with begin
+    introduce x `return_of` d ==> x `respects` d with _. begin
+      lemma_return_of_implies_exists_trace_of d x;
+      Classical.forall_intro_2 (Classical.move_requires_2 (lemma_theta_result_implies_post d));
+      assert (x `respects` d)
+    end
+  end
+
+let new_pre0 (d1:pdm 'a 'wp1) (d2:(x:'a) -> pdm 'b ('wp2 x)) : Type0 =
+  get_pre d1 /\ (forall (x:'a). x `respects` (get_fun d1) ==> get_pre (d2 x))
+
+let lemma_new_pre0_0 (d1:pdm 'a 'wp1) (d2:(x:'a) -> pdm 'b ('wp2 x)) :
+  Lemma (forall p h. hist_bind 'wp1 'wp2 p h ==> get_pre d1) = ()
+
+let lemma_new_pre0_1 (d1:pdm 'a 'wp1) (d2:(x:'a) -> pdm 'b ('wp2 x)) :
+  Lemma (forall p h. hist_bind 'wp1 'wp2 p h ==>
+  	   (forall x. x `respects` (get_fun d1) ==> get_pre (d2 x))) = ()
+
+let lemma_new_pre0 (d1:pdm 'a 'wp1) (d2:(x:'a) -> pdm 'b ('wp2 x)) :
+  Lemma (forall p h. hist_bind 'wp1 'wp2 p h ==> new_pre0 d1 d2) =
+  lemma_new_pre0_0 d1 d2;
+  lemma_new_pre0_1 d1 d2
+
+let new_pre (d1:pdm 'a 'wp1) (d2:(x:'a) -> pdm 'b ('wp2 x)) : (pre:pure_pre {forall p h. hist_bind 'wp1 'wp2 p h ==> pre}) =
+  lemma_new_pre0 d1 d2;
+  new_pre0 d1 d2
+
+[@@ "opaque_to_smt"]
+let new_pre' (d1:pdm 'a 'wp1) (d2:(x:'a) -> pdm 'b ('wp2 x)) : (pre:pure_pre {forall p h. hist_bind 'wp1 'wp2 p h ==> pre}) =
+    new_pre d1 d2
+
+let lemma1  (d1:pdm 'a 'wp1) (d2:(x:'a) -> pdm 'b ('wp2 x)) :
+    Lemma (new_pre' d1 d2 ==> get_pre d1) by (unfold_def (`new_pre'))= ()
+
+let lemma2  (d1:pdm 'a 'wp1) (d2:(x:'a) -> pdm 'b ('wp2 x)) :
+    Lemma (new_pre' d1 d2 ==> (forall x. x `respects` (get_fun d1) ==> get_pre (d2 x))) by (unfold_def (`new_pre')) = ()
+
+(*** Defining the PDM **)
+let pdm_return (a:Type) (x:a) : pdm a (hist_return x) =
+ (| True, (fun _ -> dm_return _ x) |)
+ 
+let pdm_bind (a b:Type)
+  (wp1:hist #event a) (wp2:a -> hist #event b)
+  (f:pdm a wp1) 
+  (g:(x:a) -> pdm b (wp2 x)) :
+  pdm b (hist_bind wp1 wp2) =
+  (| new_pre' f g, 
+     (fun _ -> 
+       lemma1 f g;
+       lemma_return_of_implies_respects (get_fun f);
+       let f'' = refine_dm (get_fun f) (fun x -> x `respects` (get_fun f)) in
+       dm_bind _ _ _ _ f'' (fun x -> 
+       	 lemma2 f g;
+	 get_fun (g x))) 
+   |)
+
+let pdm_subcomp (a:Type) (wp1:hist a) (wp2:hist a) (f:pdm a wp1) :
+  Pure (pdm a wp2)
+    (requires (wp2 `hist_ord` wp1))
+    (ensures fun _ -> True) =
+  (| get_pre f, (fun _ -> dm_subcomp a wp1 wp2 (get_fun f)) |)
+
+unfold
+let pdm_if_then_else 
+  (a : Type)
+  (wp1: hist a)
+  (wp2: hist a)
+  (f : pdm a wp1)
+  (g : pdm a wp2)
+  (b : bool) : Type =
+  pdm a (hist_if_then_else wp1 wp2 b)
+
+total
+reifiable
+reflectable
+effect {
+  IOwp (a:Type) (wp : hist #event a) 
+  with {
+       repr       = pdm
+     ; return     = pdm_return
+     ; bind       = pdm_bind 
+     ; subcomp    = pdm_subcomp
+     ; if_then_else = pdm_if_then_else
+     }
+}
+
+effect IO
+  (a:Type)
+  (pre : trace -> Type0)
+  (post : trace -> trace -> a -> Type0) =
+  IOwp a 
+    (fun (p:hist_post a) (h:trace) -> pre h /\ (forall lt r. post h lt r ==>  p lt r)) 
+
+let lift_pure_pdm (a : Type) 
+  (w : pure_wp a)
+  (f:(eqtype_as_type unit -> PURE a w)) : 
+  pdm a (wp_lift_pure_hist w) =
+  lemma_wp_lift_pure_hist_implies_as_requires #a #event w;
+  (| as_requires w, (fun _ -> 
+    FStar.Monotonic.Pure.elim_pure_wp_monotonicity_forall ();
+    let r = f () in
+    let r' = dm_return _ r in
+    dm_subcomp _ _ _ r' ) |)
+
+sub_effect PURE ~> IOwp = lift_pure_pdm
+  
+assume val p : prop
+assume val p' : prop
+assume val pure_lemma (_:unit) : Lemma p
+assume val some_f (_:squash p) : IO unit (fun _ -> True) (fun _ _ _ -> True)
+assume val some_f' : unit -> IO unit (requires (fun _ -> p)) (ensures fun _ _ _ -> p')
+
+let test () : IO unit (fun _ -> True) (fun _ _ _ -> True) =
+  pure_lemma ();
+  some_f ()
+
+let test'' () : IO unit (fun _ -> True) (fun _ _ _ -> True) =
+  pure_lemma ();
+  some_f ();
+  some_f' ();
+  assert p'
+
+let static_cmd
+  (cmd : io_cmds)
+  (argz : io_args cmd) :
+  IO (io_resm cmd)
+    (requires (fun h -> io_pre cmd argz h))
+    (ensures (fun h lt r ->
+        lt == [convert_call_to_event cmd argz r])) =
+  IOwp?.reflect (| True,  (fun _ -> io_call cmd argz) |)
+
+let testStatic3 (fd:file_descr) : IO unit (fun h -> is_open fd h) (fun h lt r -> ~(is_open fd (List.rev lt @ h))) =
+  let _ = static_cmd Close fd in
+  ()
+
+let testStatic2 () : IO unit (fun _ -> True) (fun _ _ _ -> True) =
+  let fd = static_cmd Openfile "../Makefile" in
+  if Some? fd then begin (** test if Openfile was successful **)
+    let msg = static_cmd Read (Some?.v fd) in
+    let _ = static_cmd Close (Some?.v fd) in
+    ()
+  end else ()
